Move encode_distributed to UnsaturatedSolinasHeuristics
As per Jade's request

src/UnsaturatedSolinasHeuristics.v
@@ -6,7 +6,6 @@ Require Import Coq.QArith.Qabs.
 Require Import Crypto.Arithmetic.Core.
 Require Import Crypto.Arithmetic.ModOps.
 Require Import Crypto.Arithmetic.Partition.
-Require Import Crypto.Arithmetic.Distribution.
 Require Import Crypto.Util.ListUtil.
 Require Import Crypto.Util.ZRange.
 Require Import Crypto.Util.Option.
@@ -20,6 +19,79 @@ Import ListNotations.
 Local Open Scope Z_scope. Local Open Scope list_scope. Local Open Scope bool_scope.
 
 Import Associational Positional.
+
+Section encode_distributed.
+  Context weight
+          (n : nat)
+          (s : Z)
+          (c : list (Z * Z))
+          {wprops : @weight_properties weight}.
+
+  Local Notation eval := (eval weight) (only parsing).
+
+  (** Sometimes we want to ensure that each limb of our encoded
+        number [x] is larger than the corresponding limb of a given
+        bound [minvalues].  We can ensure this by encoding [x -
+        minvalues] in a way that ensures each limb is non-negative,
+        and then adding back [minvalues].  We extend [minvalues] with
+        zeros for convenience, so we don't need a proof that [length
+        minvalues = n] for the proofs about [encode_distributed]. *)
+  Definition encode_distributed (minvalues : list Z) (x : Z) : list Z
+    := let minvalues := List.firstn n (minvalues ++ List.repeat 0 n) in
+       (add weight n)
+         (Partition.partition weight n ((x - Positional.eval weight n minvalues) mod (s - Associational.eval c)))
+         minvalues.
+
+  Lemma eval_encode_distributed minvalues x
+    : 0 < s - Associational.eval c <= weight n
+      -> eval n (encode_distributed minvalues x) mod (s - Associational.eval c)
+         = x mod (s - Associational.eval c).
+  Proof using wprops.
+    intros; cbv [encode_distributed]; rewrite eval_add, Partition.eval_partition by (auto; distr_length).
+    assert (forall x, x mod (s - Associational.eval c) < s - Associational.eval c) by auto with zarith.
+    rewrite (Z.mod_small (_ mod (s - _)) (weight _)) by now eauto using Z.lt_le_trans with zarith.
+    pull_Zmod; now autorewrite with zsimplify_fast.
+  Qed.
+  Hint Rewrite eval_encode_distributed : push_eval.
+  Lemma length_encode_distributed minvalues x
+    : length (encode_distributed minvalues x) = n.
+  Proof using Type. cbv [encode_distributed]; repeat distr_length. Qed.
+  Hint Rewrite length_encode_distributed : distr_length.
+  Lemma nth_default_encode_distributed_bounded'
+        (** We add an extra hypothesis that is too bulky to prove *)
+        (Hadd : forall x y, length x = n -> length y = n -> add weight n x y = map2 Z.add x y)
+        minvalues x i d' d
+        (Hmin : (i < length minvalues)%nat)
+        (Hn : (i < n)%nat)
+    : nth_default d' minvalues i <= nth_default d (encode_distributed minvalues x) i.
+  Proof using wprops.
+    cbv [encode_distributed].
+    rewrite (nth_default_in_bounds 0 d') by lia.
+    rewrite (nth_default_in_bounds 0 d) by repeat distr_length.
+    rewrite Hadd by repeat distr_length.
+    rewrite nth_default_map2 with (d1:=0) (d2:=0);
+      autorewrite with push_nth_default distr_length.
+    rewrite Nat.min_assoc, Nat.min_id, (Nat.min_l n (_ + n)) by lia.
+    break_innermost_match; try lia;
+      autorewrite with simpl_nth_default;
+      try solve [ destruct_head'_or; try lia ].
+    match goal with |- ?x <= ?y + ?x => cut (0 <= y); [ lia | ] end.
+    auto with zarith.
+  Qed.
+  (** We would like to prove this general lemma, but since we're using
+      [Positional.add] rather than [List.map2 Z.add], it's kind-of
+      annoying to prove, so we skip it. *)
+  Lemma nth_default_encode_distributed_bounded
+        minvalues x i d' d
+        (Hmin : (i < length minvalues)%nat)
+        (Hn : (i < n)%nat)
+    : nth_default d' minvalues i <= nth_default d (encode_distributed minvalues x) i.
+  Proof using wprops.
+    apply nth_default_encode_distributed_bounded'; auto.
+  Abort.
+End encode_distributed.
+Hint Rewrite @eval_encode_distributed using solve [auto; lia] : push_eval.
+Hint Rewrite @length_encode_distributed : distr_length.
 
 Notation limbwidth n s c := (inject_Z (Z.log2_up (s - Associational.eval c)) / inject_Z (Z.of_nat n))%Q.
 
